core/properties/distributivity/sampleMoore_distributivity.v
@@ -14,8 +14,8 @@
 
  
 
-Definition Moore_m1 : Model MooreMM :=
-    (Build_Model MooreMM
+Definition Moore_m1 : Model Moore.MM :=
+    (Build_Model Moore.MM
        (
         (TransitionElement (Build_Transition_t  "0")) :: 
         (TransitionElement (Build_Transition_t  "1")) :: nil
@@ -25,8 +25,8 @@ Definition Moore_m1 : Model MooreMM :=
        )
     ).
 
-Definition Moore_m2 : Model MooreMM :=
-       (Build_Model MooreMM
+Definition Moore_m2 : Model Moore.MM :=
+       (Build_Model Moore.MM
            (
                (StateElement (Build_State_t  "S0" "1")) :: 
                (StateElement (Build_State_t  "S1" "0")) ::  
