core/properties/injectivity/sampleMoore_injectivity.v
@@ -13,16 +13,16 @@
 (* Moore models as counterexample to prove injectivity of CoqTL *)
 
  
-Definition Moore_m1 : Model MooreMM :=
-(Build_Model MooreMM
+Definition Moore_m1 : Model Moore.MM :=
+(Build_Model Moore.MM
     (
         (StateElement (Build_State_t  "S0" "1")) :: nil
     )
     ( nil )
 ).
 
-Definition Moore_m2 : Model MooreMM :=
-(Build_Model MooreMM
+Definition Moore_m2 : Model Moore.MM :=
+(Build_Model Moore.MM
     (
         (StateElement (Build_State_t  "S0" "0")) :: nil
     )
